Restate prop in terms of the minimal set of temporal operators

tlc/assert/constant_prop.v
@@ -8,25 +8,23 @@ Unset Strict Implicit.
 Unset Printing Implicit Defensive.
 
 Inductive constant_prop {C} : @prop C -> Type :=
-| CAAtom a :
+| CPAtom a :
   constant_prop (Atom a)
-| CAConj A1 A2 :
-  constant_prop A1 ->
-  constant_prop A2 ->
-  constant_prop (Conj A1 A2)
-| CANeg A0 :
-  constant_prop A0 ->
-  constant_prop (Neg A0)
-| CAAlways t (x : rigid_var t) A0 :
-  constant_prop A0 ->
-  constant_prop (Always x A0).
+| CPNot p :
+  constant_prop p ->
+  constant_prop (Not p)
+| CPOr p q :
+  constant_prop p ->
+  constant_prop q ->
+  constant_prop (Or p q)
+| CPForall t (x : rigid_var t) p :
+  constant_prop p ->
+  constant_prop (Forall x p).
 
-Definition constant_prop_t {C} :=
-  {A : @prop C & constant_prop A}.
+Definition constant_prop_t {C} := {p : @prop C & constant_prop p}.
 
-Lemma constant_prop_is_interleavable {C} A
-  (CA : @constant_prop C A) :
-  interleavable_prop A.
+Lemma constant_prop_is_interleavable {C} p (CP : @constant_prop C p)
+: interleavable_prop p.
 Proof.
-  elim: CA; by constructor.
+  elim: CP; by constructor.
 Qed.
