tlc/assert/prop.v
@@ -11,203 +11,200 @@ Set Implicit Arguments.
 Unset Strict Implicit.
 Unset Printing Implicit Defensive.
 
+(* Inductive type for building first-order temporal propositions *)
 Inductive prop {C} : Type :=
 | Atom (a : @atom C)
-| Conj (A1 A2 : prop)
-| Neg (A : prop)
-| Always {t} (x : @rigid_var C t) (A : prop)
-| AlwaysF' (A : prop)
-| AlwaysP' (A : prop)
-| ExistsF' (A : prop)
-| ExistsP' (A : prop)
-| Next (A : prop)
-| Self (A : prop).
+| Not (p : prop)
+| Or (p q : prop)
+| Forall {t} (x : @rigid_var C t) (p : prop)
+| Until' (p q : prop)
+| Since' (p q : prop)
+| Self (p : prop).
 
 Bind Scope tlc_core_scope with prop.
 
 Coercion Atom : atom >-> prop.
 
+(* Notations for true and false propositions *)
+Notation True' := (Atom (@Const _ Bool true))
+  (only parsing).
+Notation False' := (Atom (@Const _ Bool false))
+  (only parsing).
+
 (* Basic notation for building propositions *)
-Notation "A1 /\ A2" :=
-  (Conj A1 A2)
-  (at level 80, right associativity) : tlc_core_scope.
-Notation "~ A" :=
-  (Neg A)
+Notation "~ p" := (Not p)
   (at level 75, right associativity) : tlc_core_scope.
-Notation "'always:' x , A" :=
-  (@Always _ _ x A)
-  (at level 65, right associativity) : tlc_core_scope.
-Notation "'alwaysf^:' A" :=
-  (AlwaysF' A)
-  (at level 65, right associativity) : tlc_core_scope.
-Notation "'alwaysp^:' A" :=
-  (AlwaysP' A)
-  (at level 65, right associativity) : tlc_core_scope.
-Notation "'existsf^:' A" :=
-  (ExistsF' A)
-  (at level 65, right associativity) : tlc_core_scope.
-Notation "'existsp^:' A" :=
-  (ExistsP' A)
-  (at level 65, right associativity) : tlc_core_scope.
-Notation "'next:' A" :=
-  (Next A)
-  (at level 65, right associativity) : tlc_core_scope.
-Notation "'self:' A" :=
-  (Self A)
-  (at level 65, right associativity) : tlc_core_scope.
-
-(* Syntactic sugar *)
-Definition Disj {C} (A1 A2 : @prop C) : @prop C :=
-  ~(~A1 /\ ~A2).
-Notation "A1 \/ A2" :=
-  (Disj A1 A2)
+Notation "p \/ q" := (Or p q)
   (at level 85, right associativity) : tlc_core_scope.
+Notation "'forall:' x , p" := (@Forall _ _ x p)
+  (at level 65, right associativity) : tlc_core_scope.
+Notation "p 'until^' q" := (Until' p q)
+  (at level 65, right associativity) : tlc_core_scope.
+Notation "p 'since^' q" := (Since' p q)
+  (at level 65, right associativity) : tlc_core_scope.
+Notation "'self:' p" := (Self p)
+  (at level 65, right associativity) : tlc_core_scope.
 
-Definition Impl {C} (A1 A2 : @prop C) : @prop C :=
-  ~A1 \/ A2.
-Notation "A1 -> A2" :=
-  (Impl A1 A2)
-  (at level 99, right associativity, A2 at level 200) : tlc_core_scope.
-
-Definition Bicond {C} (A1 A2 : @prop C) : @prop C :=
-  A1 -> A2 \/ A2 -> A1.
-Notation "A1 <-> A2" :=
-  (Bicond A1 A2)
+(* Syntactic sugar for first-order logic *)
+Definition And {C} (p q : @prop C) : @prop C := ~(~p \/ ~q).
+Notation "p /\ q" := (And p q)
+  (at level 80, right associativity) : tlc_core_scope.
+Definition If {C} (p q : @prop C) : @prop C := ~p \/ q.
+Notation "p -> q" := (If p q)
+  (at level 99, right associativity, q at level 200) : tlc_core_scope.
+Definition Iff {C} (p q : @prop C) : @prop C := p -> q \/ q -> p.
+Notation "p <-> q" := (Iff p q)
   (at level 95, no associativity) : tlc_core_scope.
-
-Definition Exists {C t} (x : rigid_var t) (A : @prop C) : @prop C :=
-  ~always: x, ~A.
-Notation "'exists:' x , A" :=
-  (@Exists _ _ x A)
+Definition Exists {C t} (x : @rigid_var C t) (p : @prop C) : @prop C :=
+  ~forall: x, ~p.
+Notation "'exists:' x , p" := (@Exists _ _ x p)
   (at level 65, right associativity) : tlc_core_scope.
 
-Definition AlwaysF {C} (A : @prop C) : @prop C :=
-  A \/ alwaysf^: A.
-Notation "'alwaysf:' A" :=
-  (AlwaysF A)
+(* Syntactic sugar for temporal logic *)
+Definition Eventually' {C} (p : @prop C) : @prop C := True' until^ p.
+Notation "'eventually^:' p" := (Eventually' p)
+  (at level 65, right associativity) : tlc_core_scope.
+Definition Once' {C} (p : @prop C) : @prop C := True' since^ p.
+Notation "'once^:' p" := (Once' p)
+  (at level 65, right associativity) : tlc_core_scope.
+Definition Henceforth' {C} (p : @prop C) : @prop C := ~eventually^: ~p.
+Notation "'henceforth^:' p" := (Henceforth' p)
+  (at level 65, right associativity) : tlc_core_scope.
+Definition AlwaysBeen' {C} (p : @prop C) : @prop C := ~once^: ~p.
+Notation "'alwaysbeen^:' p" := (AlwaysBeen' p)
+  (at level 65, right associativity) : tlc_core_scope.
+Definition Unless' {C} (p q : @prop C) : @prop C :=
+  (henceforth^: p) \/ (p until^ q).
+Notation "p 'unless^' q" :=
+  (Unless' p q)
+  (at level 65, right associativity) : tlc_core_scope.
+Definition BackTo' {C} (p q : @prop C) : @prop C :=
+  (alwaysbeen^: p) \/ (p since^ q).
+Notation "p 'backto^' q" :=
+  (BackTo' p q)
+  (at level 65, right associativity) : tlc_core_scope.
+Definition Next {C} (p : @prop C) : @prop C := False' until^ p.
+Notation "'next:' p" := (Next p)
+  (at level 65, right associativity) : tlc_core_scope.
+Definition Previous {C} (p : @prop C) : @prop C := False' since^ p.
+Notation "'previous:' p" := (Previous p)
+  (at level 65, right associativity) : tlc_core_scope.
+Definition WeakPrevious {C} (p : @prop C) : @prop C := ~previous: ~p.
+Notation "'previous~:' p" := (WeakPrevious p)
+  (at level 65, right associativity) : tlc_core_scope.
+Definition Henceforth {C} (p : @prop C) : @prop C := p /\ henceforth^: p.
+Notation "'henceforth:' p" := (Henceforth p)
+  (at level 65, right associativity) : tlc_core_scope.
+Definition AlwaysBeen {C} (p : @prop C) : @prop C := p /\ alwaysbeen^: p.
+Notation "'alwaysbeen:' p" := (AlwaysBeen p)
+  (at level 65, right associativity) : tlc_core_scope.
+Definition Eventually {C} (p : @prop C) : @prop C := p \/ eventually^: p.
+Notation "'eventually:' p" := (Eventually p)
+  (at level 65, right associativity) : tlc_core_scope.
+Definition Once {C} (p : @prop C) : @prop C := p \/ once^: p.
+Notation "'once:' p" := (Once p)
+  (at level 65, right associativity) : tlc_core_scope.
+Definition Until {C} (p q : @prop C) : @prop C := q \/ (p /\ (p until^ q)).
+Notation "p 'until' q" := (Until p q)
+  (at level 65, right associativity) : tlc_core_scope.
+Definition Since {C} (p q : @prop C) : @prop C := q \/ (p /\ (p since^ q)).
+Notation "p 'since' q" := (Since p q)
+  (at level 65, right associativity) : tlc_core_scope.
+Definition Unless {C} (p q : @prop C) : @prop C := q \/ (p /\ (p unless^ q)).
+Notation "p 'unless' q" := (Unless p q)
+  (at level 65, right associativity) : tlc_core_scope.
+Definition BackTo {C} (p q : @prop C) : @prop C := q \/ (p /\ (p backto^ q)).
+Notation "p 'backto' q" := (BackTo p q)
   (at level 65, right associativity) : tlc_core_scope.
 
-Definition AlwaysP {C} (A : @prop C) : @prop C :=
-  A \/ alwaysp^: A.
-Notation "'alwaysp:' A" :=
-  (AlwaysP A)
-  (at level 65, right associativity) : tlc_core_scope.
-
-Definition ExistsF {C} (A : @prop C) : @prop C :=
-  A \/ existsf^: A.
-Notation "'existsf:' A" :=
-  (ExistsF A)
-  (at level 65, right associativity) : tlc_core_scope.
-
-Definition ExistsP {C} (A : @prop C) : @prop C :=
-  A \/ existsp^: A.
-Notation "'existsp:' A" :=
-  (ExistsP A)
-  (at level 65, right associativity) : tlc_core_scope.
-
-Definition StrongImpl {C} (A1 A2 : @prop C) : @prop C :=
-  (alwaysf: A1) -> A2.
-Notation "A1 =>: A2" :=
-  (StrongImpl A1 A2)
+(* Additional syntactic sugar *)
+Definition Entails {C} (p q : @prop C) : @prop C := (henceforth: p) -> q.
+Notation "p =>> q" := (Entails p q)
   (at level 98, right associativity) : tlc_core_scope.
-  
-Definition StrongBicond {C} (A1 A2 : @prop C) : @prop C :=
-  ((alwaysf: A1) -> A2) /\
-  ((alwaysf: A2) -> A1).
-Notation "A1 <=>: A2" :=
-  (StrongBicond A1 A2)
+Definition Congruent {C} (p q : @prop C) : @prop C := (p =>> q) /\ (q =>> p).
+Notation "p <=> q" := (Congruent p q)
   (at level 98, right associativity) : tlc_core_scope.
-
-Definition LeadsTo {C} (A1 A2 : @prop C) : @prop C :=
-  (alwaysf: A1) -> (existsf: A2).
-Notation "A1 ~> A2" :=
-  (LeadsTo A1 A2)
+Definition LeadsTo {C} (p q : @prop C) : @prop C := p =>> eventually: q.
+Notation "p ~> q" := (LeadsTo p q)
   (at level 97, right associativity) : tlc_core_scope.
-
-Definition PrecBy {C} (A1 A2 : @prop C) : @prop C :=
-  (alwaysf: A1) -> (existsp: A2).
-Notation "A1 <~ A2" :=
-  (PrecBy A1 A2)
+Definition PrecededBy {C} (p q : @prop C) : @prop C := p =>> once: q.
+Notation "p <~ q" := (PrecededBy p q)
   (at level 97, right associativity) : tlc_core_scope.
 
 (* Extracts the types of rigid variable used in a prop *)
-Fixpoint prop_var_types {C} (A : @prop C) :=
-  match A with
+Fixpoint prop_var_types {C} (p : @prop C) :=
+  match p with
   | Atom a => term_var_types a
-  | Conj A1 A2 => union (prop_var_types A1) (prop_var_types A2)
-  | Neg A0 => prop_var_types A0
-  | Always _ _ A0 => prop_var_types A0
-  | AlwaysF' A0 => prop_var_types A0
-  | AlwaysP' A0 => prop_var_types A0
-  | ExistsF' A0 => prop_var_types A0
-  | ExistsP' A0 => prop_var_types A0
-  | Next A0 => prop_var_types A0
-  | Self A0 => prop_var_types A0
+  | Not q => prop_var_types q
+  | Or q r => union (prop_var_types q) (prop_var_types r)
+  | Forall _ _ q => prop_var_types q
+  | Until' q r => union (prop_var_types q) (prop_var_types r)
+  | Since' q r => union (prop_var_types q) (prop_var_types r)
+  | Self q => prop_var_types q
   end.
 
 (* Extracts the free rigid variables used in a prop *)
-Fixpoint prop_free_vars {C} (A : @prop C) (t : type) : seq (@rigid_var C t).
-  inversion A.
+Fixpoint prop_free_vars {C} (p : @prop C) (t : type) : seq (@rigid_var C t).
+  case: p => [a | q | q r | tx x q | q r | q r | q].
   - (* Atom *)
-    apply (@term_vars _ _ a t).
-  - (* Conj *)
-    specialize (prop_free_vars _ A1 t) as s1.
-    specialize (prop_free_vars _ A2 t) as s2.
-    apply (union s1 s2).
-  - (* Neg *)
-    apply (prop_free_vars _ A0 t).
-  - (* Always *)
-    specialize (prop_free_vars _ A0 t) as s0.
-    case Ht: (t == t0); move/eqP: Ht => Ht.
-    - (* t = t0 *)
-      subst t0.
-      apply (rem x s0).
-    - (* t <> t0 *)
-      apply s0.
-  - (* AlwaysF' *)
-    apply (prop_free_vars _ A0 t).
-  - (* AlwaysP' *)
-    apply (prop_free_vars _ A0 t).
-  - (* ExistsF' *)
-    apply (prop_free_vars _ A0 t).
-  - (* ExistsP' *)
-    apply (prop_free_vars _ A0 t).
-  - (* Next *)
-    apply (prop_free_vars _ A0 t).
+    by exact: (@term_vars _ _ a t).
+  - (* Not *)
+    by exact: (prop_free_vars _ q t).
+  - (* Or *)
+    by exact: (union (prop_free_vars _ q t) (prop_free_vars _ r t)).
+  - (* Forall *)
+    specialize (prop_free_vars _ q t) as s.
+    case Ht: (t == tx); move/eqP: Ht => Ht.
+    - (* t = tx *)
+      subst tx; by exact: (rem x s).
+    - (* t <> tx *)
+      by exact: s.
+  - (* Until' *)
+    by exact: (union (prop_free_vars _ q t) (prop_free_vars _ r t)).
+  - (* Since' *)
+    by exact: (union (prop_free_vars _ q t) (prop_free_vars _ r t)).
   - (* Self *)
-    apply (prop_free_vars _ A0 t).
+    by exact: (prop_free_vars _ q t).
 Defined.
 
 (* Extracts the rigid variables used in a term *)
-Fixpoint prop_vars {C} (A : @prop C) (t : type) :=
-  match A with
-  | Atom a => term_vars a t
-  | Conj A1 A2 => union (prop_vars A1 t) (prop_vars A2 t)
-  | Neg A0 => prop_vars A0 t
-  | Always _ _ A0 => prop_vars A0 t
-  | AlwaysF' A0 => prop_vars A0 t
-  | AlwaysP' A0 => prop_vars A0 t
-  | ExistsF' A0 => prop_vars A0 t
-  | ExistsP' A0 => prop_vars A0 t
-  | Next A0 => prop_vars A0 t
-  | Self A0 => prop_vars A0 t
-  end.
+Fixpoint prop_vars {C} (p : @prop C) (t : type) : seq (@rigid_var C t).
+  case: p => [a | q | q r | tx x q | q r | q r | q].
+  - (* Atom *)
+    by exact: (@term_vars _ _ a t).
+  - (* Not *)
+    by exact: (prop_vars _ q t).
+  - (* Or *)
+    by exact: (union (prop_vars _ q t) (prop_vars _ r t)).
+  - (* Forall *)
+    specialize (prop_vars _ q t) as s.
+    case Ht: (t == tx); move/eqP: Ht => Ht.
+    - (* t = tx *)
+      subst tx; by exact: (undup (x :: s)).
+    - (* t <> tx *)
+      by exact: s.
+  - (* Until' *)
+    by exact: (union (prop_vars _ q t) (prop_vars _ r t)).
+  - (* Since' *)
+    by exact: (union (prop_vars _ q t) (prop_vars _ r t)).
+  - (* Self *)
+    by exact: (prop_vars _ q t).
+Defined.
 
 (* Extracts the bound rigid variables used in a term *)
-Definition prop_bound_vars {C} (A : @prop C) (t : type) :=
-  filter (fun x => x \notin prop_free_vars A t) (prop_vars A t).
+Definition prop_bound_vars {C} (p : @prop C) (t : type) :=
+  filter (fun x => x \notin prop_free_vars p t) (prop_vars p t).
 
 (* Generalizes a prop by universally quantifying all free variables *)
-Definition generalize_prop {C} (A : @prop C) :=
-  foldr (fun t A => foldr Always A (prop_free_vars A t)) A (prop_var_types A).
+Definition generalize_prop {C} (p : @prop C) :=
+  foldr (fun t p => foldr Forall p (prop_free_vars p t)) p (prop_var_types p).
 
-Definition always_subst {C tx}
+Definition forall_subst {C tx}
 (prop_subst : (forall t, @substitution C t) -> @prop C)
 (s : forall t, @substitution C t)
-(x : @rigid_var C tx) (A : @prop C) : @prop C.
-
+(x : @rigid_var C tx) (p : @prop C) : @prop C.
   have x' : rigid_var tx.
-    have p (y : rigid_var tx) : bool.
+    have f (y : rigid_var tx) : bool.
       have e : term tx.
         case (s _ y) => [e' | ].
         - (* Some e' *)
@@ -216,7 +213,7 @@ Definition always_subst {C tx}
           by exact: (Rigid y).
       pose es := (term_vars e tx).
       by exact: (x \in es).
-    case (has p (filter (fun y => y != x) (prop_free_vars A tx))).
+    case (has f (filter (fun y => y != x) (prop_free_vars p tx))).
     - (* has *)
       have s' : forall t, @rigid_var C t -> option (@term C t).
       move=> ty; case H : (ty == tx); move/eqP: H => H.
@@ -232,7 +229,7 @@ Definition always_subst {C tx}
     - (* doesn't *)
       by exact: x.
 
-  (* Substitution to apply to the proposition A *)
+  (* Substitution to apply to the proposition p *)
   have s' : forall t, @rigid_var C t -> option (@term C t).
   move=> ty; case H : (ty == tx); move/eqP: H => H.
   - (* ty == tx *)
@@ -244,34 +241,28 @@ Definition always_subst {C tx}
   - (* ty != tx *)
     move=> y; by exact: (s _ y).
 
-  by exact: (Always x' (prop_subst s')).
+  by exact: (Forall x' (prop_subst s')).
 Defined.
 
 (* Substitution of terms in place of rigid variables *)
-Fixpoint prop_subst {C} (s : forall t, @substitution C t) (A : @prop C)
+Fixpoint prop_subst {C} (s : forall t, @substitution C t) (p : @prop C)
 : @prop C.
-  inversion A.
+  case: p => [a | q | q r | tx x q | q r | q r | q].
   - (* Atom *)
-    exact: (Atom (term_subst s a)).
-  - (* Conj *)
-    exact: (Conj (prop_subst _ s A1) (prop_subst _ s A2)).
-  - (* Neg *)
-    exact: (Neg (prop_subst _ s A0)).
-  - (* Always *)
-    (* This is a hack; A0 is already applied to prop_subst to satisfy the
-       fixpoint decreasing argument requirements.  However, always_subst still
-       needs A0 to substitute over *)
-    apply (always_subst (fun s => prop_subst C s A0) s x A0).
-  - (* AlwaysF' *)
-    exact: (AlwaysF' (prop_subst _ s A0)).
-  - (* AlwaysP' *)
-    exact: (AlwaysP' (prop_subst _ s A0)).
-  - (* ExistsF' *)
-    exact: (ExistsF' (prop_subst _ s A0)).
-  - (* ExistsP' *)
-    exact: (ExistsP' (prop_subst _ s A0)).
-  - (* Next *)
-    exact: (Next (prop_subst _ s A0)).
+    by exact: (Atom (term_subst s a)).
+  - (* Not *)
+    by exact: (Not (prop_subst _ s q)).
+  - (* Or *)
+    by exact: (Or (prop_subst _ s q) (prop_subst _ s r)).
+  - (* Forall *)
+    (* This is a hack; q is already applied to prop_subst to satisfy the
+       fixpoint decreasing argument requirements.  However, forall_subst still
+       needs q to substitute over *)
+    by exact: (forall_subst (fun s => prop_subst C s q) s x q).
+  - (* Until' *)
+    by exact: (Until' (prop_subst _ s q) (prop_subst _ s r)).
+  - (* Since' *)
+    by exact: (Since' (prop_subst _ s q) (prop_subst _ s r)).
   - (* Self *)
-    exact: (Self (prop_subst _ s A0)).
+    by exact: (Self (prop_subst _ s q)).
 Defined.
