tlc/assert/top_prop.v
@@ -1,47 +1,46 @@
 From mathcomp.ssreflect
 Require Import ssreflect.
 From tlc.assert
-Require Import rigid_var term prop lib interleavable_prop.
+Require Import type rigid_var term prop lib interleavable_prop.
 
 Set Implicit Arguments.
 Unset Strict Implicit.
 Unset Printing Implicit Defensive.
 
 Inductive top_prop {C} : @prop C -> Type :=
-| TACorrect t :
+| TPCorrect t :
   top_prop (Atom (App TLC.correct t))
-| TARequestEv n e :
-  top_prop (TLC.On n (TLC.Ev TLC.nil TLC.Request e))
-| TAIndicationEv n e i :
-  top_prop (TLC.On n (TLC.Ev (App (App TLC.cons i) TLC.nil) TLC.Indication e))
-| TAPeriodicEv n e :
-  top_prop (TLC.On n (TLC.Ev TLC.nil TLC.Periodic e))
-| TAConj A1 A2 :
-  top_prop A1 ->
-  top_prop A2 ->
-  top_prop (Conj A1 A2)
-| TANeg A0 :
-  top_prop A0 ->
-  top_prop (Neg A0)
-| TAAlways t (x : rigid_var t) A0 :
-  top_prop A0 ->
-  top_prop (Always x A0)
-| TAAlwaysF' A0 :
-  top_prop A0 ->
-  top_prop (AlwaysF' A0)
-| TAAlwaysP' A0 :
-  top_prop A0 ->
-  top_prop (AlwaysP' A0)
-| TAExistsF' A0 :
-  top_prop A0 ->
-  top_prop (ExistsF' A0)
-| TAExistsP' A0 :
-  top_prop A0 ->
-  top_prop (ExistsP' A0).
+| TPRequestEv n e :
+  top_prop (TLC.IsOn n (TLC.IsEvent TLC.nil TLC.Request e))
+| TPIndicationEv n e i :
+  top_prop (TLC.IsOn n
+    (TLC.IsEvent (App (App TLC.cons i) TLC.nil) TLC.Indication e))
+| TPPeriodicEv n e :
+  top_prop (TLC.IsOn n (TLC.IsEvent TLC.nil TLC.Periodic e))
+| TPNot p :
+  top_prop p ->
+  top_prop (Not p)
+| TPOr p q :
+  top_prop p ->
+  top_prop q ->
+  top_prop (Or p q)
+| TPForall t (x : rigid_var t) p :
+  top_prop p ->
+  top_prop (Forall x p)
+| TPUntil' p q :
+  p <> Atom (@Const _ Bool false) ->
+  top_prop p ->
+  top_prop q ->
+  top_prop (Until' p q)
+| TPSince' p q :
+  p <> Atom (@Const _ Bool false) ->
+  top_prop p ->
+  top_prop q ->
+  top_prop (Since' p q).
 
-Lemma top_prop_is_interleavable {C} A (TA : @top_prop C A) :
-  interleavable_prop A.
+Lemma top_prop_is_interleavable {C} p (TP : @top_prop C p)
+: interleavable_prop p.
 Proof.
-  elim: TA; try by constructor;
-  try by (rewrite /TLC.On /TLC.Ev /TLC.Eq; repeat constructor).
+  elim: TP; try by constructor;
+  try by (rewrite /TLC.IsOn /TLC.IsEvent /TLC.Eq; repeat constructor).
 Qed.
